wip

theories/Ast.v
@@ -77,34 +77,7 @@ Definition mkApps t us :=
 Definition mkApp t u := Eval cbn in mkApps t [u].
 
 
-(* one_inductive_body from declarations.ml *)
-Record inductive_body :=
-  mkinductive_body
-    { ind_name : ident;
-      ind_type : term; (* Closed arity *)
-      ind_kelim : list sort_family; (* Allowed elimination sorts *)
-      ind_ctors : list (ident * term (* Under context of arities of the mutual inductive *)
-                    * nat (* arity, w/o lets, w/o parameters *));
-      ind_projs : list (ident * term) (* names and types of projections, if any.
-                                     Type under context of params and inductive object *) }.
-
-(* mutual_inductive_body from declarations *)
-Record minductive_decl :=
-  { ind_npars : nat;
-    ind_bodies : list inductive_body ;
-    ind_universes : universe_context
-  }.
-
-(* constant_body from declarations.ml *)
-Record constant_decl :=
-  { cst_universes : universe_context;
-    cst_type : term;
-    cst_body : option term }.
-
-Inductive global_decl :=
-| ConstantDecl : kername -> constant_decl -> global_decl
-| InductiveDecl : kername -> minductive_decl -> global_decl.
-
+(** * Entries *)
 
 (** representation of mutual inductives. nearly copied from Coq/kernel/entries.mli
 *)
@@ -139,9 +112,9 @@ Inductive recursivity_kind :=
 Record definition_entry := {
   definition_entry_type : term;
   definition_entry_body : term;
-  (* definition_entry_polymorphic : bool; *)
-  (* definition_entry_universes   : universe_context; *)
-  (* definition_entry_opaque      : bool; *)
+  definition_entry_polymorphic : bool;
+  definition_entry_universes   : universe_context;
+  definition_entry_opaque      : bool;
  }.
 
 
@@ -152,31 +125,28 @@ Inductive constant_entry :=
 | ParameterEntry (p : parameter_entry)
 | DefinitionEntry (def : definition_entry).
 
-Record mutual_inductive_entry : Set := {
+Record mutual_inductive_entry := {
   mind_entry_record : option (option ident); 
   mind_entry_finite : recursivity_kind;
   mind_entry_params : list (ident * local_entry);
   mind_entry_inds : list one_inductive_entry;
   mind_entry_polymorphic : bool; 
-(*  mind_entry_universes : Univ.universe_context; *)
-  (* Should the above be used? At least we need one number indicating
-     the number of polymorphically bound definitions*)
+  mind_entry_universes : univ.universe_context;
   mind_entry_private : option bool
 }.
 
 
-(** * Environments *)
+(** * Declarations *)
 
-(* local declaration *)
+(** ** The context of De Bruijn indices *)
+
 Record context_decl := { decl_name : name ;
                          decl_body : option term ;
                          decl_type : term }.
 
 Definition vass x A := {| decl_name := x; decl_body := None; decl_type := A |}.
-Definition vdef x t A :=
-  {| decl_name := x; decl_body := Some t; decl_type := A |}.
+Definition vdef x t A := {| decl_name := x; decl_body := Some t; decl_type := A |}.
 
-(* The context of De Bruijn indices *)
 (* local ctx *)
 Definition context := list context_decl.
 
@@ -184,17 +154,40 @@ Definition snoc {A} (Γ : list A) (d : A) := d :: Γ.
 
 Notation " Γ ,, d " := (snoc Γ d) (at level 20, d at next level).
 
-(* The context of global constants *)
-Definition global_context := list global_decl.
+(** ** The context of global constants *)
+
+(* one_inductive_body from declarations.ml *)
+Record inductive_body :=
+  mkinductive_body
+    { ind_name : ident;
+      ind_type : term; (* Closed arity *)
+      ind_kelim : list sort_family; (* Allowed elimination sorts *)
+      ind_ctors : list (ident * term (* Under context of arities of the mutual inductive *)
+                    * nat (* arity, w/o lets, w/o parameters *));
+      ind_projs : list (ident * term) (* names and types of projections, if any.
+                                     Type under context of params and inductive object *) }.
+
+(* mutual_inductive_body from declarations.ml *)
+Record minductive_decl :=
+  { ind_npars : nat;
+    ind_bodies : list inductive_body ;
+    ind_universes : universe_context
+  }.
+
+(* constant_body from declarations.ml *)
+Record constant_decl :=
+  { cst_universes : universe_context;
+    cst_type : term;
+    cst_body : option term }.
+
+Inductive global_decl :=
+| ConstantDecl : kername -> constant_decl -> global_decl
+| InductiveDecl : kername -> minductive_decl -> global_decl.
 
 
+Definition global_declarations := list global_decl.
 
-Record eviron := { env_global : global_context ;
-                   env_local  : context ;
-                   env_univ   : universe_context }.
-
-
-
+Definition global_context : Type := global_declarations * uGraph.t.
 
 
 
@@ -208,12 +201,13 @@ Inductive program :=
 Definition extend_program (p : program) (d : global_decl) : program :=
   match d with
   | ConstantDecl i {| cst_universes := u; cst_type:=ty;  cst_body:=Some body |}
-    => PConstr i u (* TODO universes *) ty body p
+    => PConstr i u ty body p
   | ConstantDecl i {| cst_universes := u; cst_type:=ty;  cst_body:=None |}
     => PAxiom i u ty p
   | InductiveDecl i {| ind_npars:=n; ind_bodies := l ; ind_universes := u |}
     => PType i u n l p
   end.
+
 
 
 
