theories/Typing.v
@@ -70,7 +70,7 @@ Proof.
   unfold ident_eq. destruct string_dec; constructor; auto.
 Qed.
 
-Fixpoint lookup_env (Σ : global_context) (id : ident) : option global_decl :=
+Fixpoint lookup_env (Σ : global_declarations) (id : ident) : option global_decl :=
   match Σ with
   | nil => None
   | hd :: tl =>
@@ -78,7 +78,7 @@ Fixpoint lookup_env (Σ : global_context) (id : ident) : option global_decl :=
     else lookup_env tl id
   end.
 
-Definition declared_constant (Σ : global_context) (id : ident) decl : Prop :=
+Definition declared_constant (Σ : global_declarations) (id : ident) decl : Prop :=
   lookup_env Σ id = Some (ConstantDecl id decl).
 
 Definition declared_minductive Σ mind decl :=
@@ -129,7 +129,7 @@ Definition inds ind u (l : list inductive_body) :=
   in aux (List.length l).
 
 Program
-Definition type_of_constructor (Σ : global_context) (c : inductive * nat) (u : list Level.t) (decl : ident * term * nat)
+Definition type_of_constructor (Σ : global_declarations) (c : inductive * nat) (u : list Level.t) (decl : ident * term * nat)
            (H : declared_constructor Σ c decl) :=
   let mind := inductive_mind (fst c) in
   let '(id, trm, args) := decl in
@@ -174,7 +174,7 @@ Definition is_constructor n ts :=
 Definition iota_red npar c args brs :=
   (mkApps (snd (List.nth c brs (0, tRel 0))) (List.skipn npar args)).
 
-Inductive red1 (Σ : global_context) (Γ : context) : term -> term -> Prop :=
+Inductive red1 (Σ : global_declarations) (Γ : context) : term -> term -> Prop :=
 (** Reductions *)
 (** Beta *)
 | red_beta na t b a l :
@@ -228,11 +228,11 @@ Inductive red1 (Σ : global_context) (Γ : context) : term -> term -> Prop :=
 | cast_red_l M1 k M2 N1 : red1 Σ Γ M1 N1 -> red1 Σ Γ (tCast M1 k M2) (tCast N1 k M2)
 | cast_red_r M2 k N2 M1 : red1 Σ Γ M2 N2 -> red1 Σ Γ (tCast M1 k M2) (tCast M1 k N2)
                                        
-with reds1 (Σ : global_context) (Γ : context): list term -> list term -> Prop :=
+with reds1 (Σ : global_declarations) (Γ : context): list term -> list term -> Prop :=
 | reds1_hd hd hd' tl : red1 Σ Γ hd hd' -> reds1 Σ Γ (hd :: tl) (hd' :: tl)
 | reds1_tl hd tl tl' : reds1 Σ Γ tl tl' -> reds1 Σ Γ (hd :: tl) (hd :: tl')
 
-with redbrs1 (Σ : global_context) (Γ : context) : list (nat * term) -> list (nat * term) -> Prop :=
+with redbrs1 (Σ : global_declarations) (Γ : context) : list (nat * term) -> list (nat * term) -> Prop :=
 | redbrs1_hd n hd hd' tl : red1 Σ Γ hd hd' -> redbrs1 Σ Γ ((n, hd) :: tl) ((n, hd') :: tl)
 | redbrs1_tl hd tl tl' : redbrs1 Σ Γ tl tl' -> redbrs1 Σ Γ (hd :: tl) (hd :: tl').
 
@@ -383,162 +383,162 @@ Definition universe_family u :=
 (*   end. *)
 
 
-Reserved Notation " Σ ;;; φ ;;; Γ |- t : T " (at level 50, φ, Γ, t, T at next level).
-Reserved Notation " Σ ;;; φ ;;; Γ |- t <= u " (at level 50, φ, Γ, t, u at next level).
+Reserved Notation " Σ ;;; Γ |- t : T " (at level 50, Γ, t, T at next level).
+Reserved Notation " Σ ;;; Γ |- t <= u " (at level 50, Γ, t, u at next level).
 
 
-Inductive cumul (Σ : global_context) (φ : uGraph.t) (Γ : context) : term -> term -> Prop :=
-| cumul_refl t u : leq_term φ t u = true -> Σ ;;; φ ;;; Γ |- t <= u
-| cumul_red_l t u v : red1 Σ Γ t v -> Σ ;;; φ ;;; Γ |- v <= u -> Σ ;;; φ ;;; Γ |- t <= u
-| cumul_red_r t u v : Σ ;;; φ ;;; Γ |- t <= v -> red1 Σ Γ u v -> Σ ;;; φ ;;; Γ |- t <= u
+Inductive cumul (Σ : global_context) (Γ : context) : term -> term -> Prop :=
+| cumul_refl t u : leq_term (snd Σ) t u = true -> Σ ;;; Γ |- t <= u
+| cumul_red_l t u v : red1 (fst Σ) Γ t v -> Σ ;;; Γ |- v <= u -> Σ ;;; Γ |- t <= u
+| cumul_red_r t u v : Σ ;;; Γ |- t <= v -> red1 (fst Σ) Γ u v -> Σ ;;; Γ |- t <= u
 
-where " Σ ;;; φ ;;; Γ |- t <= u " := (@cumul Σ φ Γ t u) : type_scope.
+where " Σ ;;; Γ |- t <= u " := (@cumul Σ Γ t u) : type_scope.
 
-Definition conv Σ φ Γ T U :=
-  Σ ;;; φ ;;; Γ |- T <= U /\ Σ ;;; φ ;;; Γ |- U <= T.
+Definition conv Σ Γ T U :=
+  Σ ;;; Γ |- T <= U /\ Σ ;;; Γ |- U <= T.
 
-Notation " Σ ;;; φ ;;; Γ |- t = u " := (@conv Σ φ Γ t u) (at level 50, φ, Γ, t, u at next level) : type_scope.
+Notation " Σ ;;; Γ |- t = u " := (@conv Σ Γ t u) (at level 50, Γ, t, u at next level) : type_scope.
 
-Axiom conv_refl : forall Σ φ Γ t, Σ ;;; φ ;;; Γ |- t = t.
-Axiom cumul_refl' : forall Σ φ Γ t, Σ ;;; φ ;;; Γ |- t <= t. (* easy *)
-Axiom cumul_trans : forall Σ φ Γ t u v, Σ ;;; φ ;;; Γ |- t <= u -> Σ ;;; φ ;;; Γ |- u <= v -> Σ ;;; φ ;;; Γ |- t <= v.
+Axiom conv_refl : forall Σ Γ t, Σ ;;; Γ |- t = t.
+Axiom cumul_refl' : forall Σ Γ t, Σ ;;; Γ |- t <= t. (* easy *)
+Axiom cumul_trans : forall Σ Γ t u v, Σ ;;; Γ |- t <= u -> Σ ;;; Γ |- u <= v -> Σ ;;; Γ |- t <= v.
 
 Hint Resolve conv_refl cumul_refl' : typecheck.
 
-Conjecture congr_cumul_prod : forall Σ φ Γ na na' M1 M2 N1 N2,
-    cumul Σ φ Γ M1 N1 ->
-    cumul Σ φ (Γ ,, vass na M1) M2 N2 ->
-    cumul Σ φ Γ (tProd na M1 M2) (tProd na' N1 N2).
+Conjecture congr_cumul_prod : forall Σ Γ na na' M1 M2 N1 N2,
+    cumul Σ Γ M1 N1 ->
+    cumul Σ (Γ ,, vass na M1) M2 N2 ->
+    cumul Σ Γ (tProd na M1 M2) (tProd na' N1 N2).
 
 
 Record squash (A : Type) : Prop := { _ : A }.
 
-Inductive typing (Σ : global_context) (φ : uGraph.t) (Γ : context) : term -> term -> Type :=
+Inductive typing (Σ : global_context) (Γ : context) : term -> term -> Type :=
 | type_Rel n : forall (isdecl : n < List.length Γ),
-    Σ ;;; φ ;;; Γ |- (tRel n) : lift0 (S n) (safe_nth Γ (exist _ n isdecl)).(decl_type)
+    Σ ;;; Γ |- (tRel n) : lift0 (S n) (safe_nth Γ (exist _ n isdecl)).(decl_type)
 
-| type_Sort s s' :
-    check_lt φ s s' = true ->
-    Σ ;;; φ ;;; Γ |- (tSort s) : tSort s'
+| type_Sort l :
+    Σ ;;; Γ |- (tSort (Universe.make l)) : tSort (Universe.super l)
 
 | type_Cast c k t s :
-    Σ ;;; φ ;;; Γ |- t : tSort s ->
-    Σ ;;; φ ;;; Γ |- c : t ->
-    Σ ;;; φ ;;; Γ |- (tCast c k t) : t
+    Σ ;;; Γ |- t : tSort s ->
+    Σ ;;; Γ |- c : t ->
+    Σ ;;; Γ |- (tCast c k t) : t
 
 | type_Prod n t b s1 s2 :
-    Σ ;;; φ ;;; Γ |- t : tSort s1 ->
-    Σ ;;; φ ;;; Γ ,, vass n t |- b : tSort s2 ->
-    Σ ;;; φ ;;; Γ |- (tProd n t b) : tSort (Universe.sup s1 s2)
+    Σ ;;; Γ |- t : tSort s1 ->
+    Σ ;;; Γ ,, vass n t |- b : tSort s2 ->
+    Σ ;;; Γ |- (tProd n t b) : tSort (Universe.sup s1 s2)
 
 | type_Lambda n n' t b s1 bty :
-    Σ ;;; φ ;;; Γ |- t : tSort s1 ->
-    Σ ;;; φ ;;; Γ ,, vass n t |- b : bty ->
-    Σ ;;; φ ;;; Γ |- (tLambda n t b) : tProd n' t bty
+    Σ ;;; Γ |- t : tSort s1 ->
+    Σ ;;; Γ ,, vass n t |- b : bty ->
+    Σ ;;; Γ |- (tLambda n t b) : tProd n' t bty
 
 | type_LetIn n b b_ty b' s1 b'_ty :
-    Σ ;;; φ ;;; Γ |- b_ty : tSort s1 ->
-    Σ ;;; φ ;;; Γ |- b : b_ty ->
-    Σ ;;; φ ;;; Γ ,, vdef n b b_ty |- b' : b'_ty ->
-    Σ ;;; φ ;;; Γ |- (tLetIn n b b_ty b') : tLetIn n b b_ty b'_ty
+    Σ ;;; Γ |- b_ty : tSort s1 ->
+    Σ ;;; Γ |- b : b_ty ->
+    Σ ;;; Γ ,, vdef n b b_ty |- b' : b'_ty ->
+    Σ ;;; Γ |- (tLetIn n b b_ty b') : tLetIn n b b_ty b'_ty
 
 | type_App t l t_ty t' :
-    Σ ;;; φ ;;; Γ |- t : t_ty ->
-    typing_spine Σ φ Γ t_ty l t' ->
-    Σ ;;; φ ;;; Γ |- (tApp t l) : t'
+    Σ ;;; Γ |- t : t_ty ->
+    typing_spine Σ Γ t_ty l t' ->
+    Σ ;;; Γ |- (tApp t l) : t'
 
 | type_Const cst u : (* TODO Universes *)
-    forall decl (isdecl : declared_constant Σ cst decl),
-    Σ ;;; φ ;;; Γ |- (tConst cst u) : decl.(cst_type)
+    forall decl (isdecl : declared_constant (fst Σ) cst decl),
+    Σ ;;; Γ |- (tConst cst u) : decl.(cst_type)
 
 | type_Ind ind u :
-    forall decl (isdecl : declared_inductive Σ ind decl),
-    Σ ;;; φ ;;; Γ |- (tInd ind u) : decl.(ind_type)
+    forall decl (isdecl : declared_inductive (fst Σ) ind decl),
+    Σ ;;; Γ |- (tInd ind u) : decl.(ind_type)
 
 | type_Construct ind i u :
-    forall decl (isdecl : declared_constructor Σ (ind, i) decl),
-    Σ ;;; φ ;;; Γ |- (tConstruct ind i u) : type_of_constructor Σ (ind, i) u decl isdecl
+    forall decl (isdecl : declared_constructor (fst Σ) (ind, i) decl),
+    Σ ;;; Γ |- (tConstruct ind i u) : type_of_constructor (fst Σ) (ind, i) u decl isdecl
 
 | type_Case ind u npar p c brs args :
-    forall decl (isdecl : declared_minductive Σ (inductive_mind ind) decl),
-    forall decl' (isdecl' : declared_inductive Σ ind decl'),
+    forall decl (isdecl : declared_minductive (fst Σ) (inductive_mind ind) decl),
+    forall decl' (isdecl' : declared_inductive (fst Σ) ind decl'),
     decl.(ind_npars) = npar ->
     let pars := List.firstn npar args in
     forall pty s btys, types_of_case ind u pars p decl' = Some (pty,s,btys) ->
     List.Exists (fun sf => universe_family s = sf) decl'.(ind_kelim) ->
-    Σ ;;; φ ;;; Γ |- p : pty ->
-    Σ ;;; φ ;;; Γ |- c : mkApps (tInd ind u) args ->
-    Forall2 (fun x y => fst x = fst y /\ squash (Σ ;;; φ ;;; Γ |- snd x : snd y)) brs btys ->
-    Σ ;;; φ ;;; Γ |- tCase (ind, npar) p c brs : tApp p (List.skipn npar args ++ [c])
+    Σ ;;; Γ |- p : pty ->
+    Σ ;;; Γ |- c : mkApps (tInd ind u) args ->
+    Forall2 (fun x y => fst x = fst y /\ squash (Σ ;;; Γ |- snd x : snd y)) brs btys ->
+    Σ ;;; Γ |- tCase (ind, npar) p c brs : tApp p (List.skipn npar args ++ [c])
 
 | type_Proj p c u :
-    forall decl (isdecl : declared_projection Σ p decl) args,
-    Σ ;;; φ ;;; Γ |- c : mkApps (tInd (fst (fst p)) u) args ->
+    forall decl (isdecl : declared_projection (fst Σ) p decl) args,
+    Σ ;;; Γ |- c : mkApps (tInd (fst (fst p)) u) args ->
     let ty := snd decl in
-    Σ ;;; φ ;;; Γ |- tProj p c : substl (c :: List.rev args) ty
+    Σ ;;; Γ |- tProj p c : substl (c :: List.rev args) ty
 
 | type_Fix mfix n :
     forall (isdecl : n < List.length mfix),
     let ty := (safe_nth mfix (exist _ n isdecl)).(dtype) in
     (** TODO check well-formed fix *)
-    Σ ;;; φ ;;; Γ |- tFix mfix n : ty
+    Σ ;;; Γ |- tFix mfix n : ty
 
 | type_CoFix mfix n :
     forall (isdecl : n < List.length mfix),
     let ty := (safe_nth mfix (exist _ n isdecl)).(dtype) in
     (** TODO check well-formed cofix *)
-    Σ ;;; φ ;;; Γ |- tCoFix mfix n : ty
+    Σ ;;; Γ |- tCoFix mfix n : ty
 
 | type_Conv t A B s :
-    Σ ;;; φ ;;; Γ |- t : A ->
-    Σ ;;; φ ;;; Γ |- B : tSort s ->
-    Σ ;;; φ ;;; Γ |- A <= B ->
-    Σ ;;; φ ;;; Γ |- t : B
+    Σ ;;; Γ |- t : A ->
+    Σ ;;; Γ |- B : tSort s ->
+    Σ ;;; Γ |- A <= B ->
+    Σ ;;; Γ |- t : B
 
-where " Σ ;;; φ ;;; Γ |- t : T " := (@typing Σ φ Γ t T) : type_scope
+where " Σ ;;; Γ |- t : T " := (@typing Σ Γ t T) : type_scope
 
-with typing_spine (Σ : global_context) (φ : uGraph.t) (Γ : context) : term -> list term -> term -> Prop :=
-| type_spine_nil ty : typing_spine Σ φ Γ ty [] ty
+with typing_spine (Σ : global_context) (Γ : context) : term -> list term -> term -> Prop :=
+| type_spine_nil ty : typing_spine Σ Γ ty [] ty
 | type_spine_const hd tl na A B B' :
-    Σ ;;; φ ;;; Γ |- hd : A ->
-    typing_spine Σ φ Γ (subst0 hd B) tl B' ->
-    typing_spine Σ φ Γ (tProd na A B) (cons hd tl) B'.
+    Σ ;;; Γ |- hd : A ->
+    typing_spine Σ Γ (subst0 hd B) tl B' ->
+    typing_spine Σ Γ (tProd na A B) (cons hd tl) B'.
 
+Definition add_constraints_env u (Σ : global_context)
+  := (fst Σ, add_constraints u (snd Σ)).
 
-
-Fixpoint decompose_program (p : program) (env : uGraph.t * global_context) : uGraph.t * global_context * term :=
+Fixpoint decompose_program (p : program) (Σ : global_context) : global_context * term :=
   match p with
   | PConstr s u ty trm p =>
     let decl :=  {| cst_universes := u; cst_type := ty; cst_body := Some trm |} in
-    decompose_program p (add_constraints u (fst env), ConstantDecl s decl :: snd env)
+    decompose_program p (ConstantDecl s decl :: fst Σ, add_constraints u (snd Σ))
   | PAxiom s u ty p =>
     let decl := {| cst_universes := u; cst_type := ty; cst_body := None |} in
-    decompose_program p (add_constraints u (fst env), ConstantDecl s decl :: snd env)
+    decompose_program p (ConstantDecl s decl :: fst Σ, add_constraints u (snd Σ))
   | PType ind u m inds p =>
     let decl := {| ind_npars := m; ind_bodies := inds; ind_universes := u |} in
-    decompose_program p (add_constraints u (fst env), InductiveDecl ind decl :: snd env)
-  | PIn t => (env, t)
+    decompose_program p (InductiveDecl ind decl :: fst Σ, add_constraints u (snd Σ))
+  | PIn t => (Σ, t)
   end.
 
-Definition isType (Σ : global_context) (φ : uGraph.t) (Γ : context) (t : term) :=
-  { s : _ & Σ ;;; φ ;;; Γ |- t : tSort s }.
+Definition isType (Σ : global_context) (Γ : context) (t : term) :=
+  { s : _ & Σ ;;; Γ |- t : tSort s }.
 
-Inductive type_constructors (Σ : global_context) (φ : uGraph.t) (Γ : context) :
+Inductive type_constructors (Σ : global_context) (Γ : context) :
   list (ident * term * nat) -> Type :=
-| type_cnstrs_nil : type_constructors Σ φ Γ []
+| type_cnstrs_nil : type_constructors Σ Γ []
 | type_cnstrs_cons id t n l :
-    isType Σ φ Γ t ->
-    type_constructors Σ φ Γ l ->
+    isType Σ Γ t ->
+    type_constructors Σ Γ l ->
     (** TODO: check it has n products ending in a tRel application *)              
-    type_constructors Σ φ Γ ((id, t, n) :: l).
+    type_constructors Σ Γ ((id, t, n) :: l).
 
-Inductive type_projections (Σ : global_context) (φ : uGraph.t) (Γ : context) :
+Inductive type_projections (Σ : global_context) (Γ : context) :
   list (ident * term) -> Type :=
-| type_projs_nil : type_projections Σ φ Γ []
+| type_projs_nil : type_projections Σ Γ []
 | type_projs_cons id t l :
-    isType Σ φ Γ t ->
-    type_projections Σ φ Γ l ->
-    type_projections Σ φ Γ ((id, t) :: l).
+    isType Σ Γ t ->
+    type_projections Σ Γ l ->
+    type_projections Σ Γ ((id, t) :: l).
       
 Definition arities_context (l : list inductive_body) :=
   List.map (fun ind => vass (nNamed ind.(ind_name)) ind.(ind_type)) l.
@@ -550,55 +550,63 @@ Definition app_context (Γ Γ' : context) : context := (Γ' ++ Γ)%list.
 Notation " Γ  ,,, Γ' " := (app_context Γ Γ') (at level 25, Γ' at next level, left associativity).
 Notation "#| Γ |" := (List.length Γ) (at level 0, Γ at level 99, format "#| Γ |").
 
-Inductive type_inddecls (Σ : global_context) (φ : uGraph.t) (pars : context) (Γ : context) :
+Inductive type_inddecls (Σ : global_context) (pars : context) (Γ : context) :
   list inductive_body -> Type :=
-| type_ind_nil : type_inddecls Σ φ pars Γ []
+| type_ind_nil : type_inddecls Σ pars Γ []
 | type_ind_cons na ty cstrs projs kelim l :
     (** Arity is well-formed *)
-    isArity Σ φ [] ty ->
+    isArity Σ [] ty ->
     (** Constructors are well-typed *)
-    type_constructors Σ φ Γ cstrs ->
+    type_constructors Σ Γ cstrs ->
     (** Projections are well-typed *)
-    type_projections Σ φ (Γ ,,, pars ,, vass nAnon ty) projs ->
+    type_projections Σ (Γ ,,, pars ,, vass nAnon ty) projs ->
     (** The other inductives in the block are well-typed *)
-    type_inddecls Σ φ pars Γ l ->
+    type_inddecls Σ pars Γ l ->
     (** TODO: check kelim*)
-    type_inddecls Σ φ pars Γ (mkinductive_body na ty kelim cstrs projs :: l).
+    type_inddecls Σ pars Γ (mkinductive_body na ty kelim cstrs projs :: l).
 
-Definition type_inductive Σ φ inds :=
+Definition type_inductive Σ inds :=
   (** FIXME: should be pars ++ arities w/o params *)
-  type_inddecls Σ φ [] (arities_context inds) inds.
+  type_inddecls Σ [] (arities_context inds) inds.
                  
-Inductive fresh_global (s : string) : global_context -> Prop :=
+Inductive fresh_global (s : string) : global_declarations -> Prop :=
 | fresh_global_nil : fresh_global s nil
 | fresh_global_cons env g :
     fresh_global s env -> global_decl_ident g <> s ->
     fresh_global s (cons g env).
   
-Definition type_constant_decl Σ φ d :=
+Definition type_constant_decl Σ d :=
   match d.(cst_body) with
-  | Some trm => Σ ;;; φ ;;; [] |- trm : d.(cst_type)
-  | None => isType Σ φ [] d.(cst_type)
+  | Some trm => Σ ;;; [] |- trm : d.(cst_type)
+  | None => isType Σ [] d.(cst_type)
   end.
 
-Definition type_global_decl Σ φ decl :=
+Definition type_global_decl Σ decl :=
   match decl with  (* TODO universes *)
-  | ConstantDecl id d => type_constant_decl Σ φ d
-  | InductiveDecl ind inds => type_inductive Σ φ inds.(ind_bodies)
+  | ConstantDecl id d => type_constant_decl Σ d
+  | InductiveDecl ind inds => type_inductive Σ inds.(ind_bodies)
   end.
 
-Inductive type_global_env φ : global_context -> Type :=
-| globenv_nil : type_global_env φ []
+
+Definition contains_init_graph φ :=
+  LevelSet.In Level.prop (fst φ) /\ LevelSet.In Level.set (fst φ) /\
+  Constraint.In (Level.prop, Le, Level.set) (snd φ).
+
+Definition wf_graph φ :=
+  contains_init_graph φ /\ (no_universe_inconsistency φ = true).
+
+Inductive type_global_env φ : global_declarations -> Type :=
+| globenv_nil : wf_graph φ -> type_global_env φ []
 | globenv_decl Σ id d :
     type_global_env φ Σ ->
     fresh_global id Σ ->
-    type_global_decl Σ φ d ->
+    type_global_decl (Σ, φ) d ->
     type_global_env φ (d :: Σ).
 
-Definition type_local_decl Σ φ Γ d :=
+Definition type_local_decl Σ Γ d :=
   match d.(decl_body) with
-  | None => isType Σ φ Γ d.(decl_type)
-  | Some body => Σ ;;; φ ;;; Γ |- body : d.(decl_type)
+  | None => isType Σ Γ d.(decl_type)
+  | Some body => Σ ;;; Γ |- body : d.(decl_type)
   end.
 
 (* Fixpoint type_global_env (G : global_context) := *)
@@ -607,31 +615,31 @@ Definition type_local_decl Σ φ Γ d :=
 (*   | d :: Σ => *)
 (*     match d with *)
 (*     | ConstantDecl id d => fresh_global id Σ /\ type_global_env  *)
-Inductive type_local_env (Σ : global_context) (φ : uGraph.t) : context -> Prop :=
-| localenv_nil : type_local_env Σ φ []
+Inductive type_local_env (Σ : global_context) : context -> Prop :=
+| localenv_nil : type_local_env Σ []
 | localenv_cons Γ d :
-    type_local_env Σ φ Γ ->
-    type_local_decl Σ φ Γ d ->
-    type_local_env Σ φ (Γ ,, d).
+    type_local_env Σ Γ ->
+    type_local_decl Σ Γ d ->
+    type_local_env Σ (Γ ,, d).
 
 
 Definition type_program (p : program) (ty : term) : Prop :=
-  let '((φ, Σ), t) := decompose_program p (uGraph.init_graph, []) in
-  squash (Σ ;;; φ ;;; [] |- t : ty).
+  let '(Σ, t) := decompose_program p ([], uGraph.init_graph) in
+  squash (Σ ;;; [] |- t : ty).
 
 Quote Recursively Definition foo := 0.
 
 Ltac setenv na :=
   match goal with
-    |- ?Σ ;;; _ ;;; ?Γ |- _ : _ => set(na := Σ)
+    |- ?Σ ;;; ?Γ |- _ : _ => set(na := Σ)
   end.
 
 Ltac construct :=
   match goal with
-    |- ?Σ ;;; ?φ ;;; ?Γ |- tConstruct ?c ?i ?u : _ =>
+    |- ?Σ ;;; ?Γ |- tConstruct ?c ?i ?u : _ =>
     let H := fresh in let H' := fresh in evar(decl:(ident * term * nat)%type);
-    unshelve assert(H:declared_constructor Σ (c,i) ?decl) by repeat econstructor;
-    try (simpl; omega); assert(H':=type_Construct Σ φ Γ c i u _ H); simpl in H';
+    unshelve assert(H:declared_constructor (fst Σ) (c,i) ?decl) by repeat econstructor;
+    try (simpl; omega); assert(H':=type_Construct Σ Γ c i u _ H); simpl in H';
     clear H; apply H'
   end.
 
@@ -666,7 +674,7 @@ Definition on_decl P d :=
     Forall (fun ind => P ind.(ind_type)) ind.(ind_bodies)
   end.
 
-Inductive Forall_decls P : global_context -> Prop :=
+Inductive Forall_decls P : global_declarations -> Prop :=
 | Forall_decls_nil : Forall_decls P nil
 | Forall_decls_cons Σ d :
     Forall_decls P Σ ->
@@ -674,7 +682,7 @@ Inductive Forall_decls P : global_context -> Prop :=
     Forall_decls P (d :: Σ).
 
 Lemma term_env_ind :
-  forall P : global_context -> term -> Prop,
+  forall P : global_declarations -> term -> Prop,
     (forall Σ n, P Σ (tRel n)) ->
     (forall Σ i, P Σ (tVar i)) ->
     (forall Σ n, P Σ (tMeta n)) ->
@@ -728,7 +736,7 @@ Proof.
 Defined.
 
 Lemma term_env_ind' :
-  forall P : global_context -> term -> Prop,
+  forall P : global_declarations -> term -> Prop,
     (forall Σ n, P Σ (tRel n)) ->
     (forall Σ i, P Σ (tVar i)) ->
     (forall Σ n, P Σ (tMeta n)) ->
@@ -780,16 +788,16 @@ Definition on_decl_typing (P : term -> term -> Type) d :=
     Forall (fun ind => forall s, P ind.(ind_type) s) ind.(ind_bodies)
   end.
 
-Inductive Forall_decls_typing φ (P : global_context -> term -> term -> Type) : global_context -> Type :=
+Inductive Forall_decls_typing φ (P : global_declarations -> term -> term -> Type) : global_declarations -> Type :=
 | Forall_decls_typing_nil : Forall_decls_typing φ P nil
 | Forall_decls_typing_cons Σ d :
     Forall_decls_typing φ P Σ ->
-    on_decl_typing (fun t T => Σ ;;; φ ;;; [] |- t : T -> P Σ t T) d ->
+    on_decl_typing (fun t T => (Σ, φ) ;;; [] |- t : T -> P Σ t T) d ->
     Forall_decls_typing φ P (d :: Σ).
 
 Definition size := nat.
 
-Definition typing_size {Σ φ Γ t T} (d : Σ ;;; φ ;;; Γ |- t : T) : size.
+Definition typing_size {Σ Γ t T} (d : Σ ;;; Γ |- t : T) : size.
 Proof.
   induction d;
     match goal with
@@ -815,7 +823,7 @@ Defined.
 (*     Forall (fun ind => exists s, P ind.(ind_type) s) ind.(ind_bodies) *)
 (*   end. *)
 
-Fixpoint globenv_size (Σ : global_context) : size :=
+Fixpoint globenv_size (Σ : global_declarations) : size :=
   match Σ with
   | [] => 1
   | d :: Σ => S (globenv_size Σ)
@@ -842,36 +850,26 @@ Require Import Wellfounded Relation_Definitions.
 Require Import Relation_Operators Lexicographic_Product Wf_nat.
 Arguments lexprod [A B].
 
-Definition contains_init_graph φ :=
-  LevelSet.In Level.prop (fst φ) /\ LevelSet.In Level.set (fst φ) /\
-  Constraint.In (Level.prop, Le, Level.set) (snd φ).
+Notation wf := (fun Σ => type_global_env (snd Σ) (fst Σ)).
 
-Definition wf_graph φ :=
-  contains_init_graph φ /\ (no_universe_inconsistency φ = true).
-
-Definition wf φ Σ : Type :=
-  wf_graph φ * type_global_env φ Σ.
-
-(* FIXME we even have Prop : Set ... *)
 Conjecture wf_graph_prop_set : forall φ (H : wf_graph φ),
     check_lt φ Universe.type0m Universe.type1 = true /\
     check_lt φ Universe.type0 Universe.type1 = true.
 
-Definition env_prop (P : forall Σ φ Γ t T, Set) :=
-  forall Σ φ (wfΣ : wf φ Σ) Γ t T, Σ ;;; φ ;;; Γ |- t : T ->
-    Forall_decls_typing φ (fun Σ t ty => P Σ φ [] t ty) Σ *
-    P Σ φ Γ t T.
+Definition env_prop (P : forall Σ Γ t T, Set) :=
+  forall Σ (wfΣ : wf Σ) Γ t T, Σ ;;; Γ |- t : T ->
+    Forall_decls_typing (snd Σ) (fun Σ' t ty => P (Σ', snd Σ) [] t ty) (fst Σ) *
+    P Σ Γ t T.
 
 Lemma env_prop_typing P : env_prop P ->
-  forall Σ φ (wf : wf φ Σ) (Γ : context) (t T : term),
-    Σ;;; φ ;;; Γ |- t : T -> P Σ φ Γ t T.
+  forall Σ (wf : wf Σ) (Γ : context) (t T : term),
+    Σ ;;; Γ |- t : T -> P Σ Γ t T.
 Proof. intros. now apply X. Qed.
 
 Lemma env_prop_sigma P : env_prop P ->
-  forall Σ φ (wf : wf φ Σ),
-    Forall_decls_typing φ (fun (Σ0 : global_context) (t0 ty : term) => P Σ0 φ [] t0 ty) Σ.
-Proof. intros. eapply X. apply wf0. apply (type_Sort Σ φ [] Universe.type0).
-       eapply wf_graph_prop_set. eapply wf0.
+  forall Σ (wf : wf Σ),
+    Forall_decls_typing (snd Σ) (fun Σ0 (t0 ty : term) => P (Σ0, snd Σ) [] t0 ty) (fst Σ).
+Proof. intros. eapply X. apply wf. apply (type_Sort Σ [] Level.prop).
 Defined.
 
 (** An induction principle ensuring the Σ declarations enjoy the same properties. *)
@@ -879,114 +877,113 @@ Defined.
 (*   TODO: thread the property on local contexts as well, avoiding to redo work at binding constructs. *)
 (*  *)
 Lemma typing_ind_env :
-  forall (P : global_context -> uGraph.t -> context -> term -> term -> Set),
-    (forall Σ φ (wfΣ : wf φ Σ) (Γ : context) (n : nat) (isdecl : n < #|Γ|),
-        P Σ φ Γ (tRel n)
+  forall (P : global_context -> context -> term -> term -> Set),
+    (forall Σ (wfΣ : wf Σ) (Γ : context) (n : nat) (isdecl : n < #|Γ|),
+        P Σ Γ (tRel n)
           (lift0 (S n) (decl_type (safe_nth Γ (exist (fun n0 : nat => n0 < #|Γ|) n isdecl))))) ->
-    (forall Σ φ (wfΣ : wf φ Σ) (Γ : context) (s s': universe), check_lt φ s s' = true -> P Σ φ Γ (tSort s) (tSort s')) ->
-    (forall Σ φ (wfΣ : wf φ Σ) (Γ : context) (c : term) (k : cast_kind) (t : term) (s : universe),
-        Σ ;;; φ ;;; Γ |- t : tSort s -> P Σ φ Γ t (tSort s) -> Σ ;;; φ ;;; Γ |- c : t -> P Σ φ Γ c t -> P Σ φ Γ (tCast c k t) t) ->
-    (forall Σ φ (wfΣ : wf φ Σ) (Γ : context) (n : name) (t b : term) (s1 s2 : universe),
-        Σ ;;; φ ;;; Γ |- t : tSort s1 ->
-        P Σ φ Γ t (tSort s1) ->
-        Σ ;;; φ ;;; Γ,, vass n t |- b : tSort s2 ->
-        P Σ φ (Γ,, vass n t) b (tSort s2) -> P Σ φ Γ (tProd n t b) (tSort (Universe.sup s1 s2))) ->
-    (forall Σ φ (wfΣ : wf φ Σ) (Γ : context) (n n' : name) (t b : term) (s1 : universe) (bty : term),
-        Σ ;;; φ ;;; Γ |- t : tSort s1 ->
-        P Σ φ Γ t (tSort s1) ->
-        Σ ;;; φ ;;; Γ,, vass n t |- b : bty -> P Σ φ (Γ,, vass n t) b bty -> P Σ φ Γ (tLambda n t b) (tProd n' t bty)) ->
-    (forall Σ φ (wfΣ : wf φ Σ) (Γ : context) (n : name) (b b_ty b' : term) (s1 : universe) (b'_ty : term),
-        Σ ;;; φ ;;; Γ |- b_ty : tSort s1 ->
-        P Σ φ Γ b_ty (tSort s1) ->
-        Σ ;;; φ ;;; Γ |- b : b_ty ->
-        P Σ φ Γ b b_ty ->
-        Σ ;;; φ ;;; Γ,, vdef n b b_ty |- b' : b'_ty ->
-        P Σ φ (Γ,, vdef n b b_ty) b' b'_ty -> P Σ φ Γ (tLetIn n b b_ty b') (tLetIn n b b_ty b'_ty)) ->
-    (forall Σ φ (wfΣ : wf φ Σ) (Γ : context) (t : term) (l : list term) (t_ty t' : term),
-        Σ ;;; φ ;;; Γ |- t : t_ty -> P Σ φ Γ t t_ty -> typing_spine Σ φ Γ t_ty l t' -> P Σ φ Γ (tApp t l) t') ->
+    (forall Σ (wfΣ : wf Σ) (Γ : context) (l : Level.t), P Σ Γ (tSort (Universe.make l)) (tSort (Universe.super l))) ->
+    (forall Σ (wfΣ : wf Σ) (Γ : context) (c : term) (k : cast_kind) (t : term) (s : universe),
+        Σ ;;; Γ |- t : tSort s -> P Σ Γ t (tSort s) -> Σ ;;; Γ |- c : t -> P Σ Γ c t -> P Σ Γ (tCast c k t) t) ->
+    (forall Σ (wfΣ : wf Σ) (Γ : context) (n : name) (t b : term) (s1 s2 : universe),
+        Σ ;;; Γ |- t : tSort s1 ->
+        P Σ Γ t (tSort s1) ->
+        Σ ;;; Γ,, vass n t |- b : tSort s2 ->
+        P Σ (Γ,, vass n t) b (tSort s2) -> P Σ Γ (tProd n t b) (tSort (Universe.sup s1 s2))) ->
+    (forall Σ (wfΣ : wf Σ) (Γ : context) (n n' : name) (t b : term) (s1 : universe) (bty : term),
+        Σ ;;; Γ |- t : tSort s1 ->
+        P Σ Γ t (tSort s1) ->
+        Σ ;;; Γ,, vass n t |- b : bty -> P Σ (Γ,, vass n t) b bty -> P Σ Γ (tLambda n t b) (tProd n' t bty)) ->
+    (forall Σ (wfΣ : wf Σ) (Γ : context) (n : name) (b b_ty b' : term) (s1 : universe) (b'_ty : term),
+        Σ ;;; Γ |- b_ty : tSort s1 ->
+        P Σ Γ b_ty (tSort s1) ->
+        Σ ;;; Γ |- b : b_ty ->
+        P Σ Γ b b_ty ->
+        Σ ;;; Γ,, vdef n b b_ty |- b' : b'_ty ->
+        P Σ (Γ,, vdef n b b_ty) b' b'_ty -> P Σ Γ (tLetIn n b b_ty b') (tLetIn n b b_ty b'_ty)) ->
+    (forall Σ (wfΣ : wf Σ) (Γ : context) (t : term) (l : list term) (t_ty t' : term),
+        Σ ;;; Γ |- t : t_ty -> P Σ Γ t t_ty -> typing_spine Σ Γ t_ty l t' -> P Σ Γ (tApp t l) t') ->
 
-    (forall Σ φ (wfΣ : wf φ Σ) (Γ : context) (cst : ident) u (decl : constant_decl),
-        declared_constant Σ cst decl ->
-        Forall_decls_typing φ (fun Σ t ty => P Σ φ [] t ty) Σ ->
-        P Σ φ Γ (tConst cst u) (cst_type decl)) ->
+    (forall Σ (wfΣ : wf Σ) (Γ : context) (cst : ident) u (decl : constant_decl),
+        declared_constant (fst Σ) cst decl ->
+        Forall_decls_typing (snd Σ) (fun Σ' t ty => P (Σ', snd Σ) [] t ty) (fst Σ) ->
+        P Σ Γ (tConst cst u) (cst_type decl)) ->
 
-        (forall Σ φ (wfΣ : wf φ Σ) (Γ : context) (ind : inductive) u (decl : inductive_body),
-        declared_inductive Σ ind decl -> P Σ φ Γ (tInd ind u) (ind_type decl)) ->
-       (forall Σ φ (wfΣ : wf φ Σ) (Γ : context) (ind : inductive) (i : nat) u (decl : ident * term * nat)
-          (isdecl : declared_constructor Σ (ind, i) decl),
-        P Σ φ Γ (tConstruct ind i u) (type_of_constructor Σ (ind, i) u decl isdecl)) ->
-       (forall Σ φ (wfΣ : wf φ Σ) (Γ : context) (ind : inductive) u (npar : nat) (p c : term) (brs : list (nat * term))
+        (forall Σ (wfΣ : wf Σ) (Γ : context) (ind : inductive) u (decl : inductive_body),
+        declared_inductive (fst Σ) ind decl -> P Σ Γ (tInd ind u) (ind_type decl)) ->
+       (forall Σ (wfΣ : wf Σ) (Γ : context) (ind : inductive) (i : nat) u (decl : ident * term * nat)
+          (isdecl : declared_constructor (fst Σ) (ind, i) decl),
+        P Σ Γ (tConstruct ind i u) (type_of_constructor (fst Σ) (ind, i) u decl isdecl)) ->
+       (forall Σ (wfΣ : wf Σ) (Γ : context) (ind : inductive) u (npar : nat) (p c : term) (brs : list (nat * term))
           (args : list term) (decl : minductive_decl),
-        declared_minductive Σ (inductive_mind ind) decl ->
+        declared_minductive (fst Σ) (inductive_mind ind) decl ->
         forall decl' : inductive_body,
-        declared_inductive Σ ind decl' ->
+        declared_inductive (fst Σ) ind decl' ->
         ind_npars decl = npar ->
         let pars := firstn npar args in
         forall (pty : term) (s : universe) (btys : list (nat * term)),
         types_of_case ind u pars p decl' = Some (pty, s, btys) ->
         Exists (fun sf => universe_family s = sf) (ind_kelim decl') ->
-        Σ ;;; φ ;;; Γ |- p : pty ->
-        P Σ φ Γ p pty ->
-        Σ ;;; φ ;;; Γ |- c : mkApps (tInd ind u) args ->
-        P Σ φ Γ c (mkApps (tInd ind u) args) ->
-        Forall2 (fun x y : nat * term => fst x = fst y /\ squash (Σ ;;; φ ;;; Γ |- snd x : snd y)) brs btys ->
-        P Σ φ Γ (tCase (ind, npar) p c brs) (tApp p (skipn npar args ++ [c]))) ->
-       (forall Σ φ (wfΣ : wf φ Σ) (Γ : context) (p : projection) (c : term) u (decl : ident * term),
-        declared_projection Σ p decl ->
+        Σ ;;; Γ |- p : pty ->
+        P Σ Γ p pty ->
+        Σ ;;; Γ |- c : mkApps (tInd ind u) args ->
+        P Σ Γ c (mkApps (tInd ind u) args) ->
+        Forall2 (fun x y : nat * term => fst x = fst y /\ squash (Σ ;;; Γ |- snd x : snd y)) brs btys ->
+        P Σ Γ (tCase (ind, npar) p c brs) (tApp p (skipn npar args ++ [c]))) ->
+       (forall Σ (wfΣ : wf Σ) (Γ : context) (p : projection) (c : term) u (decl : ident * term),
+        declared_projection (fst Σ) p decl ->
         forall args : list term,
-        Σ ;;; φ ;;; Γ |- c : mkApps (tInd (fst (fst p)) u) args ->
-        P Σ φ Γ c (mkApps (tInd (fst (fst p)) u) args) ->
-        let ty := snd decl in P Σ φ Γ (tProj p c) (substl (c :: rev args) ty)) ->
-       (forall Σ φ (wfΣ : wf φ Σ) (Γ : context) (mfix : list (def term)) (n : nat) (isdecl : n < #|mfix|),
+        Σ ;;; Γ |- c : mkApps (tInd (fst (fst p)) u) args ->
+        P Σ Γ c (mkApps (tInd (fst (fst p)) u) args) ->
+        let ty := snd decl in P Σ Γ (tProj p c) (substl (c :: rev args) ty)) ->
+       (forall Σ (wfΣ : wf Σ) (Γ : context) (mfix : list (def term)) (n : nat) (isdecl : n < #|mfix|),
         let ty := dtype (safe_nth mfix (exist (fun n0 : nat => n0 < #|mfix|) n isdecl)) in
-        P Σ φ Γ (tFix mfix n) ty) ->
-       (forall Σ φ (wfΣ : wf φ Σ) (Γ : context) (mfix : list (def term)) (n : nat) (isdecl : n < #|mfix|),
+        P Σ Γ (tFix mfix n) ty) ->
+       (forall Σ (wfΣ : wf Σ) (Γ : context) (mfix : list (def term)) (n : nat) (isdecl : n < #|mfix|),
         let ty := dtype (safe_nth mfix (exist (fun n0 : nat => n0 < #|mfix|) n isdecl)) in
-        P Σ φ Γ (tCoFix mfix n) ty) ->
-       (forall Σ φ (wfΣ : wf φ Σ) (Γ : context) (t A B : term) (s : universe),
-        Σ ;;; φ ;;; Γ |- t : A ->
-                       P Σ φ Γ t A -> Σ ;;; φ ;;; Γ |- B : tSort s -> P Σ φ Γ B (tSort s) -> Σ ;;; φ ;;; Γ |- A <= B -> P Σ φ Γ t B) ->
+        P Σ Γ (tCoFix mfix n) ty) ->
+       (forall Σ (wfΣ : wf Σ) (Γ : context) (t A B : term) (s : universe),
+        Σ ;;; Γ |- t : A ->
+                       P Σ Γ t A -> Σ ;;; Γ |- B : tSort s -> P Σ Γ B (tSort s) -> Σ ;;; Γ |- A <= B -> P Σ Γ t B) ->
 
        env_prop P.
 Proof.
   unfold env_prop.
-  intros P X X0 X1 X2 X3 X4 X5 X6 X7 X8 X9 X10 X11 X12 X13 Σ φ wfΣ Γ t T H.
-  pose (@Fix_F ({ Σ : _ & {φ : _ & { wfΣ : wf φ Σ & { Γ : context & { t : term & { T : term & Σ ;;; φ ;;; Γ |- t : T }}} } }})
-               (lexprod (MR lt (fun x => globenv_size x))
-                            (fun Σ => MR lt (fun x => typing_size (projT2 (projT2 (projT2 (projT2 (projT2 x))))))))).
-  set(foo := existT _ Σ (existT _ φ (existT _ wfΣ (existT _ Γ (existT _ t (existT _ _ H))))) : { Σ : _ & {φ : _ & { wfΣ : wf φ Σ & { Γ : context & { t : term & { T : term & Σ ;;; φ ;;; Γ |- t : T }}} } }}).
+  intros P X X0 X1 X2 X3 X4 X5 X6 X7 X8 X9 X10 X11 X12 X13 Σ wfΣ Γ t T H.
+  pose (@Fix_F ({ Σ : _ & { wfΣ : wf Σ & { Γ : context & { t : term & { T : term & Σ ;;; Γ |- t : T }}} }})
+               (lexprod (MR lt (fun Σ => globenv_size (fst Σ)))
+                            (fun Σ => MR lt (fun x => typing_size (projT2 (projT2 (projT2 (projT2 x)))))))).
+  set(foo := existT _ Σ (existT _ wfΣ (existT _ Γ (existT _ t (existT _ _ H)))) : { Σ : _ & { wfΣ : wf Σ & { Γ : context & { t : term & { T : term & Σ ;;; Γ |- t : T }}} }}).
   change Σ with (projT1 foo).
-  change φ with (projT1 (projT2 foo)).
-  change Γ with (projT1 (projT2 (projT2 (projT2 foo)))).
-  change t with (projT1 (projT2 (projT2 (projT2 (projT2 foo))))).
-  change T with (projT1 (projT2 (projT2 (projT2 (projT2 (projT2 foo)))))).
+  change Γ with (projT1 (projT2 (projT2 foo))).
+  change t with (projT1 (projT2 (projT2 (projT2 foo)))).
+  change T with (projT1 (projT2 (projT2 (projT2 (projT2 foo))))).
   revert foo.
   match goal with
     |- let foo := _ in @?P foo => specialize (p (fun x => P x))
   end.
   forward p; [ | apply p; apply wf_lexprod; intros; apply measure_wf; apply lt_wf].
   clear p.
-  clear Σ φ wfΣ Γ t T H.
-  intros (Σ&φ&wfΣ&Γ&t&t0&H). simpl.
+  clear Σ wfΣ Γ t T H.
+  intros (Σ&wfΣ&Γ&t&t0&H). simpl.
   intros IH. unfold MR in IH. simpl in IH.
   split.
-  destruct Σ.
+  destruct Σ as [Σ φ]. destruct Σ.
   constructor.
-  destruct wfΣ as [wfG wfΣ]. inversion_clear wfΣ.
+  cbn in wfΣ; inversion_clear wfΣ.
   constructor.
-  refine (let IH' := IH (existT _ Σ (existT _ φ (existT _ (wfG, X14) (existT _ Γ (existT _ (tSort Universe.type0m ) (existT _ (tSort Universe.type1) (type_Sort _ _ _ Universe.type0m Universe.type1 _))))))) in _).
-  simpl in IH'. forward IH'. constructor 1. simpl. omega.
-  apply IH'.
+  specialize (IH (existT _ (Σ, φ) (existT _ X14 (existT _ Γ (existT _ (tSort Universe.type0m ) (existT _ _ (type_Sort _ _ Level.prop))))))).
+  simpl in IH. forward IH. constructor 1. simpl. omega.
+  apply IH.
   destruct g; simpl.
   destruct cst_body.
   simpl.
   intros.
-  specialize (IH (existT _ Σ (existT _ φ (existT _ (wfG, X14) (existT _ _ (existT _ _ (existT _ _ X16))))))).
+  specialize (IH (existT _ (Σ, φ) (existT _ X14 (existT _ _ (existT _ _ (existT _ _ X16)))))).
   simpl in IH.
   forward IH. constructor 1. simpl; omega.
   apply IH.
   intros.
-  specialize (IH (existT _ Σ (existT _ φ (existT _ (wfG, X14) (existT _ _ (existT _ _ (existT _ _ X16))))))).
+  specialize (IH (existT _ (Σ, φ) (existT _ X14 (existT _ _ (existT _ _ (existT _ _ X16)))))).
   simpl in IH.
   forward IH. constructor 1. simpl; omega.
   apply IH.
@@ -994,18 +991,18 @@ Proof.
   induction (ind_bodies m). constructor.
   constructor; auto.
   intros.
-  specialize (IH (existT _ Σ (existT _ φ (existT _ (wfG, X14) (existT _ _ (existT _ _ (existT _ _ X16))))))).
+  specialize (IH (existT _ (Σ, φ) (existT _ X14 (existT _ _ (existT _ _ (existT _ _ X16)))))).
   simpl in IH.
   forward IH. constructor 1. simpl; omega.
   apply IH.
 
-  assert (forall Γ t T (Hty : Σ ;;; φ ;;; Γ |- t : T),
+  assert (forall Γ t T (Hty : Σ ;;; Γ |- t : T),
              typing_size Hty <
              typing_size H ->
-             Forall_decls_typing φ (fun (Σ : global_context) (t ty : term) => P Σ φ [] t ty) Σ *
-             P Σ φ Γ t T).
+             Forall_decls_typing (snd Σ) (fun Σ' (t ty : term) => P (Σ', snd Σ) [] t ty) (fst Σ) *
+             P Σ Γ t T).
   intros.
-  specialize (IH (existT _ Σ (existT _ φ (existT _ wfΣ (existT _ _ (existT _ _ (existT _ _ Hty))))))).
+  specialize (IH (existT _ Σ (existT _ wfΣ (existT _ _ (existT _ _ (existT _ _ Hty)))))).
   simpl in IH.
   forward IH.
   constructor 2. simpl. apply H0.
@@ -1020,7 +1017,6 @@ Proof.
   unshelve eapply X14; simpl; auto with arith.
   setoid_rewrite Nat.max_comm at 2.
   rewrite Nat.max_comm, <- Nat.max_assoc. auto with arith.
-  simpl in X14. refine (let H0' := X14 [] _ _ (type_Sort _ _ _ Universe.type0m Universe.type1 _) in _).
-  simpl in H0'. forward H0'; auto. apply H0'.
-  Unshelve. all: apply wf_graph_prop_set; first [assumption|apply wfΣ].
+  specialize (X14 [] _ _ (type_Sort _ _ Level.prop)).
+  simpl in X14. forward X14; auto. apply X14.
 Qed.
